

CS229 Problem Set #0 Solution

Jaeyun Kim

December 31, 2025

1. Gradients and Hessians

(a)

$$\nabla f(x) = \nabla \left(\frac{1}{2} x^\top A x + b^\top x \right) = \nabla \left(\frac{1}{2} x^\top A x \right) + \nabla (b^\top x)$$

Let's verify the gradient of the quadratic form.

$$\nabla \left(\frac{1}{2} x^\top A x \right) = \frac{1}{2} \nabla \left(\sum_{i=1}^n x_i \sum_{j=1}^n A_{ij} x_j \right) = \frac{1}{2} \nabla \left(\sum_{i=1}^n \sum_{j=1}^n A_{ij} x_i x_j \right)$$

Now, let's look at the k -th component of the gradient by taking the partial derivative with respect to x_k

$$\frac{\partial}{\partial x_k} \left(\frac{1}{2} \sum_{i=1}^n \sum_{j=1}^n A_{ij} x_i x_j \right) = \frac{1}{2} \sum_{i=1}^n \sum_{j=1}^n A_{ij} \frac{\partial}{\partial x_k} (x_i x_j)$$

We consider three cases for the indices in the summation:

1. Case 1: $i = k$ and $j \neq k$
2. Case 2: $i \neq k$ and $j = k$
3. Case 3: $i = k$ and $j = k$

Then, the derivative is:

$$\begin{aligned} \frac{1}{2} \sum_{i=1}^n \sum_{j=1}^n A_{ij} \frac{\partial}{\partial x_k} (x_i x_j) &= \frac{1}{2} \left(\sum_{j \neq k} A_{kj} x_j + \sum_{i \neq k} A_{ik} x_i + \frac{\partial}{\partial x_k} (A_{kk} x_k^2) \right) \\ &= \frac{1}{2} \left(\sum_{j \neq k} A_{kj} x_j + \sum_{i \neq k} A_{ik} x_i + 2A_{kk} x_k \right) \\ &= \frac{1}{2} \left[\left(\sum_{j \neq k} A_{kj} x_j + A_{kk} x_k \right) + \left(\sum_{i \neq k} A_{ik} x_i + A_{kk} x_k \right) \right] \\ &= \frac{1}{2} \left(\sum_{j=1}^n A_{kj} x_j + \sum_{i=1}^n A_{ik} x_i \right) \\ &= \frac{1}{2} \left((Ax)_k + (A^\top x)_k \right) \end{aligned}$$

Therefore, $\nabla(\frac{1}{2}x^\top Ax) = \frac{1}{2}(Ax + A^\top x) = Ax$ (since A is a symmetric matrix)

Next, for the linear term:

$$\nabla(b^\top x) = \nabla \sum_{i=1}^n b_i x_i = b$$

Therefore, combining both results:

$$\nabla f(x) = Ax + b$$

(b)

$$\begin{aligned} \nabla f(x) &= \nabla g(h(x)) \\ &= \begin{bmatrix} \frac{\partial}{\partial x_1} g(h(x)) \\ \vdots \\ \frac{\partial}{\partial x_n} g(h(x)) \end{bmatrix} \\ &= \begin{bmatrix} g'(h(x)) \frac{\partial h(x)}{\partial x_1} \\ \vdots \\ g'(h(x)) \frac{\partial h(x)}{\partial x_n} \end{bmatrix} \\ &= g'(h(x)) \nabla h(x) \end{aligned}$$

(c)

$$\begin{aligned} \nabla^2 f(x) &= \begin{bmatrix} \frac{\partial}{\partial x_1} \left| \frac{\partial \nabla f(x)}{\partial x_1} \right| & \frac{\partial}{\partial x_2} \left| \frac{\partial \nabla f(x)}{\partial x_1} \right| & \dots & \frac{\partial}{\partial x_n} \left| \frac{\partial \nabla f(x)}{\partial x_1} \right| \\ \vdots & \vdots & \ddots & \vdots \end{bmatrix} \\ &= \begin{bmatrix} \frac{\partial}{\partial x_1} \left| \frac{\partial (Ax+b)}{\partial x_1} \right| & \frac{\partial}{\partial x_2} \left| \frac{\partial (Ax+b)}{\partial x_1} \right| & \dots & \frac{\partial}{\partial x_n} \left| \frac{\partial (Ax+b)}{\partial x_1} \right| \\ \vdots & \vdots & \ddots & \vdots \end{bmatrix} \\ &= \begin{bmatrix} A^{(1)} & A^{(2)} & \dots & A^{(n)} \\ \vdots & \vdots & \ddots & \vdots \end{bmatrix} \\ &= A \end{aligned}$$

(d)

Let $h(x) = a^\top x$

- **Gradient:** $\nabla f(x) = \nabla g(h(x)) = g'(h(x)) \nabla h(x) = g'(a^\top x) a$

• **Hessian:**

$$\begin{aligned}
 \text{Let } h(x) &= a^\top x \\
 \frac{\partial^2 g(h(x))}{\partial x_i \partial x_j} &= \frac{\partial}{\partial x_j} g'(h(x)) \frac{\partial h(x)}{\partial x_i} \\
 &= g''(h(x)) \frac{\partial h(x)}{\partial x_j} \frac{\partial h(x)}{\partial x_i} \\
 &= g''(a^\top x) a_j a_i
 \end{aligned}$$

Therefore, the Hessian matrix of $f(x)$ is

$$\nabla^2 f(x) = g''(a^\top x) \begin{bmatrix} a_1 a_1 & \dots & a_1 a_n \\ \vdots & \ddots & \vdots \\ a_n a_1 & \dots & a_n a_n \end{bmatrix} = g''(a^\top x) a a^\top$$

2. Positive definite matrices

(a)

$$x^\top A x = x^\top z z^\top x = (z^\top x)^\top (z^\top x) = \|z^\top x\|^2 \geq 0 \quad \therefore A \succeq 0$$

(b)

$$\begin{aligned}
 \text{Null}(A) &= \{x \mid Ax = 0\} = \{x \mid z^\top x = 0\} \quad (\because z \neq \vec{0}) \\
 \text{Nullity}(A) &= \dim(\{x \mid z^\top x = 0\}) = n - 1 \\
 \text{Rank}(A) &= 1 \quad \because (\text{rank-nullity theorem})
 \end{aligned}$$

(c)

$$\begin{aligned}
 x^\top B A B^\top x &= (B^\top x)^\top A (B^\top x) \geq 0 \quad (\because A \succeq 0) \\
 \therefore B A B^\top &\succeq 0
 \end{aligned}$$

3. Eigenvectors, eigenvalues, and the spectral theorem

(a)

$$\begin{aligned}
 A &= T \Lambda T^{-1} \\
 AT &= T \Lambda \\
 \begin{bmatrix} | & | & \dots & | \\ A t^{(1)} & A t^{(2)} & \dots & A t^{(n)} \\ | & | & & | \end{bmatrix} &= \begin{bmatrix} | & | & \dots & | \\ \lambda_1 t^{(1)} & \lambda_2 t^{(2)} & \dots & \lambda_n t^{(n)} \\ | & | & & | \end{bmatrix} \\
 \therefore A t^{(i)} &= \lambda_i t^{(i)}
 \end{aligned}$$

(b)

Since U is an orthogonal matrix, $UU^\top = I$

$$\begin{aligned} A &= U\Lambda U^\top \\ AU &= U\Lambda \\ \begin{bmatrix} | & | & & | \\ Au^{(1)} & Au^{(2)} & \dots & Au^{(n)} \\ | & | & & | \end{bmatrix} &= \begin{bmatrix} | & | & & | \\ \lambda_1 u^{(1)} & \lambda_2 u^{(2)} & \dots & \lambda_n u^{(n)} \\ | & | & & | \end{bmatrix} \end{aligned}$$

$$\therefore Au^{(i)} = \lambda_i u^{(i)} \implies u^{(i)} \text{ is an eigenvector of } A$$

(c)

$$\begin{aligned} x^\top Ax &= x^\top U\Lambda U^\top x \\ &= (U^\top x)^\top \Lambda (U^\top x) \geq 0 \quad (\forall x \in \mathbb{R}^n, \text{ since } A \succeq 0) \end{aligned}$$

Let $c = U^\top x$. Since U^\top is an orthogonal matrix, columns of U^\top span \mathbb{R}^n . Therefore, c can be any vector in \mathbb{R}^n .

$$c^\top \Lambda c = \sum_{i=1}^n c_i^2 \lambda_i \geq 0 \quad (\forall c \in \mathbb{R}^n).$$

For any $j \in \{1, \dots, n\}$, choose c such that $c_j = 1$ and $c_k = 0$ for $j \neq k$. Then,

$$\begin{aligned} c^\top \Lambda c &= \sum_{i=1}^n c_i^2 \lambda_i = \lambda_j \geq 0. \\ \therefore \lambda_i(A) &\geq 0 \quad \text{for each } i \end{aligned}$$